\documentclass{article}
\usepackage{geometry}
\usepackage{amsmath}
\usepackage{graphicx}
\usepackage{xcolor}
\title{Mathematical Induction}
\author{}
\date{}

\begin{document}
	4.4.2(c): 
	\newline
	Prove that for any positive integer n, \\
	$\Sigma^{n}_{j=1}$ $j^3$ = $(\frac{n(n+1)}{2})^2$ \\
	case 1: n = 1 \\
	$\Sigma^{n}_{j=1}$ $j^3$ = $1^3$ = 1
	and $(\frac{1(1+1)}{2})^2$ = $(\frac{1 \cdot 2}{2})^2$ = $1^2$ = 1 \\
	case 2: n = k+1 \\
	$\Sigma^{n}_{j=1}$ $j^3$ = $(\frac{n(n+1)}{2})^2$ \\
	$\color{red}{\Sigma^{k+1}_{j=1} j^3 = (\frac{(k+1)(k+2)}{2})^2}$ \\
	$\Sigma^{k+1}_{j=1}$ $j^3$ = $\Sigma^{k}_{j=1}$ $j^3$ + $(k+1)^3$ \\
	$\Sigma^{k+1}_{j=1}$ $j^3$ = $(\frac{k(k+1)}{2})^2$ + $(k+1)^3$ \\
	$(\frac{k(k+1)}{2})^2$ + $(k+1)^3$ =  $\frac{k^2(k+1)^2}{4}$ + $(k+1)^3$ \\
	= $(k+1)^2$($\frac{k^2}{4}$)($\frac{4k}{4}$)($\frac{4}{4}$) = $(k+1)^2$($\frac{k^2+4k+4}{4})$ \\
	= $(k+1)^2$($\frac{(k+2)^2}{4}$)
	= $\frac{(k+1)^2(k+2)^2}{4}$ \\
	$\color{red}{\Sigma^{k+1}_{j=1} j^3 = (\frac{(k+1)(k+2)}{2})^2}$ \\
	\newline
	4.5.1(e): \\
	Prove that for any positive integer n, 2 evenly divides $n^2$ - 5n + 2 \\
	Case1: n is even \\
	n $\equiv$ 0 (mod 2)  \\
	1. $n^2 \equiv 0^2 \equiv 0 \; (mod \; 2)$ \\
	2. 5n $\equiv$ 5 $\cdot$ 0 $\equiv$ 0 (mod 2) \\
	3. $n^2 -5n + 2 \equiv 0 - 0 + 2 \equiv 2 \equiv 0 \; (mod \; 2)$ \\
	making $n^2 -5n + 2=$ even when n is even \\
	\newline
	Case2: n is odd \\
	n $\equiv$ 1 (mod 2)  \\
	1. $n^2 \equiv 1^2 \equiv 1 (mod 2)$ \\
	2. 5n $\equiv$ 5 $\cdot$ 1 $\equiv$ 5  $\equiv$ 1 (mod 2) \\
	3. $n^2 -5n + 2 \equiv 1 - 1 + 2 \equiv 2 \equiv 0 \; (mod \; 2)$ \\
	making $n^2 -5n + 2$ odd when n is odd \\
	\newline
	Therefore, for any positive integer n, $n^2$ - 5n + 2 is even, proving that 2 evenly divides $n^2$ - 5n + 2 
	is divisible by 2 for any positive integer n. \\
	\newline
	\newline
	\newline
	\newline
	\newline
	\newline
	\newline
	\newline
	\newline
	\newline
	\newline
	\newline
	
	4.4.3(c): \\
	Prove that for n $\geq$ 1, \\
	$\Sigma^{n}_{j=1}$ $\frac{1}{j^2}$ $\leq$ 2 - $\frac{1}{n}$\\
	Consider f(x) = $\frac{1}{x^2}$ \\
	$\int_{1}^{n+1} \frac{1}{x^2} dx$ $<$ $\Sigma^{n}_{j=1} \frac{1}{j^2}$ $<$ 1 + $\int_{1}^{n} \frac{1}{x^2} dx$ \\
	$\int \frac{1}{x^2} dx$ = -$\frac{1}{x}$ + C \\
	$\int_{1}^{n+1} \frac{1}{x^2} \, dx = \left[ -\frac{1}{x} \right]_{1}^{n+1} = -\frac{1}{n+1} + 1 = 1 - \frac{1}{n+1}$ \\
	$\int_{1}^{n} \frac{1}{x^2} \, dx = \left[ -\frac{1}{x} \right]_{1}^{n} = -\frac{1}{n} + 1 = 1 - \frac{1}{n}$ \\
	\newline
	From the integrals, we now get \\
	$1 - \frac{1}{n+1} < \sum_{j=1}^{n} \frac{1}{j^2} < 1 + \left( 1 - \frac{1}{n} \right) = 2 - \frac{1}{n}$ \\
	\newline
	thus for all n $\geq$ 1:\\
	$\sum_{j=1}^{n} \frac{1}{j^2} < 2 - \frac{1}{n}$ \\
\end{document}